1

Sequent.thy
@@ -5,73 +5,57 @@ theory Sequent
   imports Symbolic_Regular_Algebra_Model 
 begin
 
-section \<open>Terms and ('a, 'b, 'c) formulae\<close>
+section \<open>Terms and 'a formulae\<close>
 
 text \<open>
-\label{sec:terms} The datatypes of terms and ('a, 'b, 'c) formulae are defined as follows:
+\label{sec:terms} The datatypes of terms and 'a formulae are defined as follows:
 \<close>
 
-datatype 'a bterm = Var nat | App 'a "('a) bterm list" 
+datatype bterm = Var nat | Conc bterm bterm
 
-datatype ('a, 'b, 'c) form = 
-    EqAtom "'a bterm" "'a bterm"                      
-  | EqPred "'a bterm" 'b "'a bterm list"      
-  | EqConc "'a bterm" "'a bterm" "'a bterm"
-  | NeqAtom "'a bterm" "'a bterm" 
-  | NeqPred "'a bterm" 'b "'a bterm list"                     
-  | Member "'a bterm" "'c rexp"
-  | Nmember "'a bterm" "'c rexp"
-  | Dis "('a, 'b, 'c) form" "('a, 'b, 'c) form"                     
-  | Con "('a, 'b, 'c) form" "('a, 'b, 'c) form"                      
-  | Neg "('a, 'b, 'c) form"     
+datatype 'a form = 
+    EqAtom "bterm" "bterm"                      
+  | NeqAtom "bterm" "bterm" 
+  | Member "bterm" "'a rexp"
+  | Nmember "bterm" "'a rexp"
+  | Dis "'a form" "'a form"                     
+  | Con "'a form" "'a form"                      
+  | Neg "'a form"     
 
 
 primrec
-  evalt :: \<open>(nat \<Rightarrow> 'c) \<Rightarrow> ('a \<Rightarrow> 'c list \<Rightarrow> 'c) \<Rightarrow> 'a bterm \<Rightarrow> 'c\<close> and
-  evalts :: \<open>(nat \<Rightarrow> 'c) \<Rightarrow> ('a \<Rightarrow> 'c list \<Rightarrow> 'c) \<Rightarrow> 'a bterm list \<Rightarrow> 'c list\<close> where
-  \<open>evalt e f (Var n) = e n\<close>
-| \<open>evalt e f (App a ts) = f a (evalts e f ts)\<close>
-| \<open>evalts e f [] = []\<close>
-| \<open>evalts e f (t # ts) = evalt e f t # evalts e f ts\<close>
+  evalt :: \<open>(nat \<Rightarrow> 'a) \<Rightarrow> ('a \<Rightarrow> 'a \<Rightarrow> 'a) \<Rightarrow>  bterm \<Rightarrow> 'a\<close>  where
+  \<open>evalt e f (Var n) = e n\<close> |
+  \<open>evalt e f (Conc m n) = f (evalt e f m) (evalt e f n)\<close>
 
+primrec eval :: \<open>(nat \<Rightarrow> 'a) \<Rightarrow>  ('a  \<Rightarrow> 'a  \<Rightarrow> 'a)  \<Rightarrow>  'a form \<Rightarrow> bool\<close> where
+  "eval e f (EqAtom x y) = (evalt e f x = evalt e f y)" 
+| "eval e f (NeqAtom x y) = (evalt e f x \<noteq> evalt e f y)" 
+| "eval e f (Member x r) = ([evalt e f x] \<in> lang r)"
+| "eval e f (Nmember x r) = ([evalt e f x] \<in> (UNIV - lang r))"
+| "eval e f (Dis m n) = (eval e f m \<or> eval e f n)"
+| "eval e f (Con m n) = (eval e f m \<and> eval e f n)"
+| "eval e f (Neg m) = (\<not> eval e f m)"
 
-primrec eval :: \<open>(nat \<Rightarrow> 'c) \<Rightarrow> ('a \<Rightarrow> 'c list \<Rightarrow> 'c) \<Rightarrow>
-  ('b \<Rightarrow> 'c list \<Rightarrow> 'c \<Rightarrow> bool)  \<Rightarrow>
-  ('c  \<Rightarrow> 'c \<Rightarrow> 'c  \<Rightarrow> bool)  \<Rightarrow> 
-  ('a, 'b, 'c) form \<Rightarrow> bool\<close> where
-  "eval e f g c (EqAtom x y) = (evalt e f x = evalt e f y)" 
-| "eval e f g c (EqPred x p ts) = g p (evalts e f ts) (evalt e f x)" 
-| "eval e f g c (EqConc x m n) = (c (evalt e f x) (evalt e f m) (evalt e f n))"
-| "eval e f g c (NeqAtom x y) = (evalt e f x \<noteq> evalt e f y)" 
-| "eval e f g c (NeqPred x p ts) = (\<not> g p (evalts e f ts) (evalt e f x))"  
-| "eval e f g c (Member x r) = ([evalt e f x] \<in> lang r)"
-| "eval e f g c (Nmember x r) = ([evalt e f x] \<notin> lang r)"
-| "eval e f g c (Dis m n) = (eval e f g c m \<or> eval e f g c n)"
-| "eval e f g c (Con m n) = (eval e f g c m \<and> eval e f g c n)"
-| "eval e f g c (Neg m) = (\<not> eval e f g c m)"
+definition model :: \<open>(nat \<Rightarrow> 'a) \<Rightarrow> ('a  \<Rightarrow> 'a \<Rightarrow> 'a )  \<Rightarrow>  'a form list \<Rightarrow> 'a form \<Rightarrow> bool\<close> ("_,_,_ \<Turnstile> _" [50,50] 50) where
+  \<open>(e,f,ps \<Turnstile> p) = (list_all (eval e f) ps \<longrightarrow> eval e f p)\<close>
 
-definition model :: \<open>(nat \<Rightarrow> 'c) \<Rightarrow> ('a \<Rightarrow> 'c list \<Rightarrow> 'c) \<Rightarrow> ('b \<Rightarrow> 'c list \<Rightarrow> 'c  \<Rightarrow> bool) \<Rightarrow>
-    ('c  \<Rightarrow> 'c \<Rightarrow> 'c  \<Rightarrow> bool)  \<Rightarrow>  ('a, 'b, 'c) form list \<Rightarrow> ('a, 'b, 'c) form \<Rightarrow> bool\<close> ("_,_,_,_,_ \<Turnstile> _" [50,50] 50) where
-  \<open>(e,f,g,c,ps \<Turnstile> p) = (list_all (eval e f g c) ps \<longrightarrow> eval e f g c p)\<close>
-
-
-fun empty_intersection_list :: "'c rexp list \<Rightarrow> bool" where 
+fun empty_intersection_list :: "'a rexp list \<Rightarrow> bool" where 
   "empty_intersection_list fs = (List.foldl (\<inter>) (lang (hd fs)) (map lang (tl fs)) = {})"
 
-fun subset_intersect_list :: "'c rexp \<Rightarrow> 'c rexp list \<Rightarrow> bool" where 
+fun subset_intersect_list :: "'a rexp \<Rightarrow> 'a rexp list \<Rightarrow> bool" where 
   "subset_intersect_list r fs = (List.foldl (\<inter>) (lang (hd fs)) (map lang (tl fs)) \<subseteq> lang r)"
 
-fun eq_len_intersect :: "'c rexp \<Rightarrow> 'c rexp list \<Rightarrow> bool" where 
+fun eq_len_intersect :: "'a rexp \<Rightarrow> 'a rexp list \<Rightarrow> bool" where 
   "eq_len_intersect r fs = (List.foldl (\<inter>) (lang (hd fs)) (map lang (tl fs)) = lang r \<and> length fs > 1)"
 
-inductive One_SC :: \<open>('a, 'b, 'c) form list \<Rightarrow> bool\<close> (\<open>\<turnstile> _\<close> 0) where
-  AlphaCon:      \<open>\<turnstile> A # B # G \<Longrightarrow> \<turnstile> Con A B # G\<close>
-| AlphaNegOr:    \<open>\<turnstile> Neg A # Neg B # G \<Longrightarrow> \<turnstile> Neg (Dis A B) # G\<close>
-| AlphaOr:       \<open>\<turnstile> A # G \<Longrightarrow> \<turnstile> B # G \<Longrightarrow> \<turnstile> Dis A B # G\<close>
-| AlphaNegAnd:   \<open>\<turnstile> Neg A # G \<Longrightarrow> \<turnstile> Neg B # G \<Longrightarrow> \<turnstile> Neg (Con A B) # G\<close>
+inductive One_SC :: \<open>'a form list \<Rightarrow> bool\<close> (\<open>\<turnstile> _\<close> 0) where
+  AlphaCon:      \<open>\<turnstile> A # B # G \<Longrightarrow> \<turnstile> Dis A B # G\<close>
+| AlphaNegOr:    \<open>\<turnstile> Neg A # Neg B # G \<Longrightarrow> \<turnstile> Neg (Con A B) # G\<close>
+| AlphaOr:       \<open>\<turnstile> A # G \<Longrightarrow> \<turnstile> B # G \<Longrightarrow> \<turnstile> Con A B # G\<close>
+| AlphaNegAnd:   \<open>\<turnstile> Neg A # G \<Longrightarrow> \<turnstile> Neg B # G \<Longrightarrow> \<turnstile> Neg (Dis A B) # G\<close>
 | AlphaNegNeg:   \<open>\<turnstile> A # G \<Longrightarrow> \<turnstile> Neg (Neg A) # G\<close>
 | NotMember:     \<open>regexp_compl e ec \<Longrightarrow> \<turnstile> (Member x ec) # G \<Longrightarrow> \<turnstile> (Nmember x e) # G\<close>
-| NEq :          \<open>\<turnstile> NeqAtom x y # (EqPred y f ts) # G \<Longrightarrow> \<turnstile> (NeqPred x f ts) # G\<close>
 | Cut:           \<open>regexp_compl e ec \<Longrightarrow> \<turnstile> Member x e # G \<Longrightarrow> \<turnstile> Member x ec # G \<Longrightarrow>  \<turnstile> G\<close>
 | EqProp:        \<open>\<turnstile> Member x e # EqAtom x y # Member y e # G \<Longrightarrow> \<turnstile> Member x e # EqAtom x y # G\<close>
 | NeqSubsume:    \<open>regexp_empty e1 e2 \<Longrightarrow> \<turnstile> Member x e1 # Member y e2 # G \<Longrightarrow> \<turnstile> Member x e1 # NeqAtom x y # Member y e2 # G\<close>
@@ -80,10 +64,10 @@ inductive One_SC :: \<open>('a, 'b, 'c) form list \<Rightarrow> bool\<close> (\<
 | Close:         \<open>empty_intersection_list fs \<Longrightarrow> \<turnstile> (map (\<lambda>r. Member x r) fs) @ G\<close>
 | Subsume:       \<open>subset_intersect_list e fs \<Longrightarrow> \<turnstile> (map (\<lambda>r. Member x r) (f # fs)) @ G \<Longrightarrow> \<turnstile> Member x e # (map (\<lambda>r. Member x r) (f#fs)) @ G\<close>
 | Intersect:     \<open>eq_len_intersect e fs \<Longrightarrow> \<turnstile> Member x e # G  \<Longrightarrow>  \<turnstile> (map (\<lambda>r. Member x r) (f#fs)) @ G\<close>
-| Fwd_PropConc:  \<open>lang e = lang (Times e1 e2) \<Longrightarrow> \<turnstile> Member x e # EqConc x m n # Member m e1 # Member n e2 # G \<Longrightarrow> \<turnstile> EqConc x m n # Member x e1 # Member x e2 # G \<close>
+(*| Fwd_PropConc:  \<open>lang e = lang (Times e1 e2) \<Longrightarrow> \<turnstile> Member x e # EqAtom x y # Member m e1 # Member n e2 # G \<Longrightarrow> \<turnstile> EqAtom x y # Member x e1 # Member x e2 # G \<close>
 | Fwd_ElimConc:  \<open>lang e = lang (Times e1 e2) \<and> is_singleton (lang e) \<Longrightarrow> is_singleton (lang e) \<Longrightarrow> \<turnstile> Member x e # Member m e1 # Member n e2 # G \<Longrightarrow>  \<turnstile> EqConc x m n # Member x e1 # Member x e2 # G\<close>
-| Bwd_Prop:      \<open>lang e = lang (Times e1 e2) \<Longrightarrow> \<turnstile> Member x e # EqConc x m n # Member m e1 # Member n e2 # G \<Longrightarrow> \<turnstile> EqConc x m n # Member x e # G \<close>
-
+| Bwd_Prop:      \<open>lang e = lang (Times e1 e2) \<Longrightarrow> \<turnstile> Member x e # EqAtom x y # Member m e1 # Member n e2 # G \<Longrightarrow> \<turnstile> EqAtom x y # Member x e # G \<close>
+*)
 lemma \<open>\<turnstile> (map (\<lambda>r. Member x r) [Atom (1::nat), Atom 2]) @ G\<close>
   apply(rule Close)
   apply auto
@@ -92,12 +76,51 @@ lemma \<open>\<turnstile> (map (\<lambda>r. Member x r) [Atom (1::nat), Atom 2])
 
 subsection \<open>Soundness\<close>
 
-lemma SC_soundness: \<open>\<turnstile> G \<Longrightarrow> \<exists>p \<in> set G. eval e f g c p\<close>
-  apply (induct G arbitrary: f g c rule: One_SC.induct)
-  subgoal for A B G f g c 
-  apply simp 
+lemma SC_soundness: \<open>\<turnstile> G \<Longrightarrow> \<exists>p \<in> set G. eval e f p\<close>
+  apply (induct G rule: One_SC.induct)
+  subgoal for A B G 
+    apply auto 
+    done 
+  subgoal for A B G 
+    apply auto 
+    done
+  subgoal for A G B
+    apply auto
+    done
+  subgoal for A B G
+    apply auto
+    done
+  subgoal for A G 
+    apply auto
+    done
+  subgoal for ea ec x G
+    apply auto 
+    done
+  subgoal for ea ec x G
+    apply auto
+    done 
+  subgoal for x ea y G
+    apply auto
     sorry
-  sorry
+  subgoal for e1 e2 x y G
+    apply auto
+    done
+  subgoal for ea x Eq y G
+    apply auto 
+    sorry
+  subgoal for ea ec x y G Neq
+    apply auto
+    sorry
+  subgoal for fs x G
+    apply auto
+    sorry
+  subgoal for ea fs x fa G
+    apply auto
+    done
+  subgoal for ea fs x G fa
+    apply auto
+    sorry
+  done
 
 
 subsection \<open>Completeness\<close>
